Safety: proved forward to backward simulation in the context of error preserving

common/SmallstepSafe.v
@@ -181,3 +181,333 @@ Arguments Backward_simulation_preserve_error {_ _ ccA _ _ ccB L1 L2 err_state1 e
 
 Definition backward_simulation_preserve_error {liA1 liA2} ccA {liB1 liB2} ccB L1 L2 err_state1 err_state2 :=
   inhabited (@bsimp_components liA1 liA2 ccA liB1 liB2 ccB L1 L2 err_state1 err_state2).
+
+(** * Forward simulation to the error preserving backward simulation *)
+
+(* Most of the proof are the same as the forward_to_backward in Smallstep.v *)
+
+Record lts_sound_err {liA liB st} (L: lts liA liB st) (err: st -> Prop) : Prop :=
+  Sound_error {
+      sd_err_nostep: forall s,
+        err s ->
+        Nostep L s;
+
+      sd_final_noerr: forall s r,
+        final_state L s r ->
+        err s ->
+        False;
+
+      sd_external_noerr: forall s q,
+        at_external L s q ->
+        err s ->
+        False;        
+    }.
+
+Definition sound_err {liA liB} (L: semantics liA liB) err :=
+  forall se,
+  lts_sound_err (L se) (err se).
+
+Section FORWARD_TO_BACKWARD.
+
+Context {liA1 liA2} (ccA: callconv liA1 liA2).
+Context {liB1 liB2} (ccB: callconv liB1 liB2).
+Context (se1 se2: Genv.symtbl) (wB: ccworld ccB).
+Context {state1 state2} (L1: lts liA1 liB1 state1) (L2: lts liA2 liB2 state2).
+Context {index order match_states} (FS: fsim_properties ccA ccB se1 se2 wB L1 L2 index order match_states).
+Hypothesis order_wf: well_founded order.
+Hypothesis Hse: match_senv ccB wB se1 se2.
+Hypothesis L1_receptive: lts_receptive L1 se1.
+Hypothesis L2_determinate: lts_determinate L2 se2.
+
+Context (err_state1: state1 -> Prop) (err_state2: state2 -> Prop).
+
+Hypothesis L2_sound_err: lts_sound_err L2 err_state2.
+
+Hypothesis err_preservation: forall i s1 s2,
+    match_states i s1 s2 ->
+    err_state1 s1 ->
+    exists s2' : state2, Star L2 s2 E0 s2' /\ err_state2 s2'.
+
+(* f2b_partial_transition is a useful predicate to exploit the
+transition in source and target *)
+
+Let f2b_transitions := @f2b_transitions _ _ ccA _ _ ccB se1 se2 wB _ _ L1 L2 index match_states.
+Inductive f2b_partial_transitions: state1 -> state2 -> Prop :=
+| f2b_trans_normal: forall s1 s2,
+    f2b_transitions s1 s2 ->
+    f2b_partial_transitions s1 s2
+| f2b_trans_err: forall s1 s1' s2 s2' i,
+    (* handle stuttering in L1 *)
+    Star L1 s1 E0 s1' ->
+    match_states i s1' s2 ->
+    err_state1 s1' ->
+    Star L2 s2 E0 s2' ->
+    err_state2 s2' ->
+    f2b_partial_transitions s1 s2.
+
+Lemma f2b_partial_progress:
+  forall i s1 s2, match_states i s1 s2 -> partial_safe L1 err_state1 s1 -> f2b_partial_transitions s1 s2.
+Proof.
+  intros i0; pattern i0. apply well_founded_ind with (R := order); auto.
+  intros i REC s1 s2 MATCH SAFE.
+  destruct (SAFE s1) as [[[r FINAL] | [[q EXTERN] | [t [s1' STEP1]]]]| ERR]. apply star_refl.
+  - (* final state reached *)
+    edestruct @fsim_match_final_states as (r2 & Hr & Hfinal); eauto.
+    eapply f2b_trans_normal. eapply f2b_trans_final; eauto.
+    apply star_refl.
+  - (* external call reached *)
+    edestruct @fsim_match_external as (w & q2 & Hq & Hat & Hse' & Hafter); eauto.
+    eapply f2b_trans_normal. eapply f2b_trans_ext; eauto.
+    apply star_refl.
+  - (* L1 can make one step *)
+    exploit (fsim_simulation FS); eauto. intros [i' [s2' [A MATCH']]].
+    assert (B: Plus L2 s2 t s2' \/ (s2' = s2 /\ t = E0 /\ order i' i)).
+    intuition auto.
+    destruct (star_inv H0); intuition auto.
+    clear A. destruct B as [PLUS2 | [EQ1 [EQ2 ORDER]]].
+    + eapply f2b_trans_normal. eapply f2b_trans_step; eauto. apply star_refl.
+    + subst. exploit REC; eauto. eapply star_partial_safe; eauto. apply star_one; auto.
+      intros TRANS. inv TRANS. inv H.
+      * eapply f2b_trans_normal. eapply f2b_trans_final; eauto. eapply star_step; eauto.
+      * eapply f2b_trans_normal. eapply f2b_trans_ext; eauto. eapply star_left; eauto.
+      * eapply f2b_trans_normal. eapply f2b_trans_step; eauto. eapply star_left; eauto.
+      (* error state  *)
+      * eapply f2b_trans_err; eauto. eapply star_left; eauto.
+  (* L1 is in the error state *)
+  - exploit err_preservation; eauto. intros (s2' & STAR & ERR2).
+    eapply f2b_trans_err; eauto. eapply star_refl. 
+Qed.
+
+(* simulation relation used in backward simulation *)
+
+Let f2b_match_states := @f2b_match_states _ _ _ _ _ _ L1 L2 index match_states.
+
+Inductive f2b_partial_match_states : f2b_index -> state1 -> state2 -> Prop :=
+| f2b_pmatch_normal: forall i s1 s2
+    (MATCH: f2b_match_states i s1 s2),
+    f2b_partial_match_states i s1 s2
+| f2b_pmatch_err: forall n s1 s2 s2b s2a i
+    (Err1: err_state1 s1)
+    (STAR: Star L2 s2b E0 s2)
+    (STARN: starN (step L2) (globalenv L2) n s2 E0 s2a)
+    (Err2: err_state2 s2a)
+    (MATCH: match_states i s1 s2b),
+    f2b_partial_match_states (F2BI_before n) s1 s2.
+
+Lemma f2b_simulation_step:
+  forall s2 t s2', Step L2 s2 t s2' ->
+  forall i s1, f2b_partial_match_states i s1 s2 -> partial_safe L1 err_state1 s1 ->
+  exists i', exists s1',
+    (Plus L1 s1 t s1' \/ (Star L1 s1 t s1' /\ f2b_order i' i))
+     /\ f2b_partial_match_states i' s1' s2'.
+Proof.
+  intros s2 t s2' STEP2 i s1 MATCH SAFE.
+  inv MATCH. inv MATCH0.
+- (* 1. At matching states *)
+  exploit f2b_partial_progress; eauto. intros TRANS; inv TRANS. inv H0.
+  + (* 1.1  L1 can reach final state and L2 is at final state: impossible! *)
+    exploit (sd_final_nostep L2_determinate); eauto. contradiction.
+  + (* 1.1b  Same, with external states *)
+    exploit (sd_at_external_nostep L2_determinate); eauto. contradiction.
+  + (* 1.2  L1 can make 0 or several steps; L2 can make 1 or several matching steps. *)
+    inv H3.
+    exploit @f2b_determinacy_inv. 1-2: eauto. eexact H0. eexact STEP2.
+    intros [[EQ1 [EQ2 EQ3]] | [NOT1 [NOT2 MT]]].
+    * (* 1.2.1  L2 makes a silent transition *)
+      destruct (silent_or_not_silent t2).
+      (* 1.2.1.1  L1 makes a silent transition too: perform transition now and go to "after" state *)
+      subst. simpl in *. destruct (star_starN H6) as [n STEPS2].
+      exists (F2BI_after n); exists s1''; split.
+      left. eapply plus_right; eauto.
+      eapply f2b_pmatch_normal.
+      eapply f2b_match_after'; eauto.
+      (* 1.2.1.2 L1 makes a non-silent transition: keep it for later and go to "before" state *)
+      subst. simpl in *. destruct (star_starN H6) as [n STEPS2].
+      exists (F2BI_before n); exists s1'; split.
+      right; split. auto. constructor.
+      eapply f2b_pmatch_normal.
+      econstructor. eauto. auto. apply star_one; eauto. eauto. eauto.
+    * (* 1.2.2 L2 makes a non-silent transition, and so does L1 *)
+      exploit not_silent_length. eapply (sr_traces L1_receptive); eauto. intros [EQ | EQ].
+      congruence.
+      subst t2. rewrite E0_right in H2.
+      (* Use receptiveness to equate the traces *)
+      exploit (sr_receptive L1_receptive); eauto. intros [s1''' STEP1].
+      exploit @fsim_simulation_not_E0. eauto. eexact STEP1. auto. eauto.
+      intros [i''' [s2''' [P Q]]]. inv P.
+      (* Exploit determinacy *)
+      exploit not_silent_length. eapply (sr_traces L1_receptive); eauto. intros [EQ | EQ].
+      subst t0. simpl in *. exploit @sd_determ_1. eauto. eexact STEP2. eexact H3.
+      intros. elim NOT2. inv H8. auto.
+      subst t2. rewrite E0_right in *.
+      assert (s4 = s2'). eapply sd_determ_2; eauto. subst s4.
+      (* Perform transition now and go to "after" state *)
+      destruct (star_starN H7) as [n STEPS2]. exists (F2BI_after n); exists s1'''; split.
+      left. eapply plus_right; eauto.
+      eapply f2b_pmatch_normal.
+      eapply f2b_match_after'; eauto.
+      
+  (* L1 and L2 step to an error state *)
+  + inv H3.
+    (* L2 make 0 or several matching steps *)
+    * (* impossible because error state cannot make step *)
+      exfalso. eapply sd_err_nostep; eauto.
+    * exploit @f2b_determinacy_inv. 1-2: eauto. eexact H5. eexact STEP2.
+      intros [[EQ1 [EQ2 EQ3]] | [NOT1 [NOT2 MT]]].
+      -- subst.
+         destruct (silent_or_not_silent t2); simpl in H7; try congruence. subst.
+         (* L1 makes 0 transition and update the index to (before n) *)
+         destruct (star_starN H6) as [n STEPS2].
+         exists (F2BI_before n), s1'; split.
+         right; split. auto. constructor.
+         eapply f2b_pmatch_err; eauto. eapply star_one; eauto.
+      -- exploit Eapp_E0_inv; eauto.
+         intros (A1 & A2). subst. congruence.
+         
+- (* 2. Before *)
+  inv H2. congruence.
+  exploit @f2b_determinacy_inv. 1-2: eauto. eexact H4. eexact STEP2.
+  intros [[EQ1 [EQ2 EQ3]] | [NOT1 [NOT2 MT]]].
+  + (* 2.1 L2 makes a silent transition: remain in "before" state *)
+    subst. simpl in *. exists (F2BI_before n0); exists s1; split.
+    right; split. apply star_refl. constructor. lia.
+    eapply f2b_pmatch_normal.
+    econstructor; eauto. eapply star_right; eauto.
+  + (* 2.2 L2 make a non-silent transition *)
+    exploit not_silent_length. eapply (sr_traces L1_receptive); eauto. intros [EQ | EQ].
+    congruence.
+    subst. rewrite E0_right in *.
+    (* Use receptiveness to equate the traces *)
+    exploit (sr_receptive L1_receptive); eauto. intros [s1''' STEP1].
+    exploit @fsim_simulation_not_E0. eauto. eexact STEP1. auto. eauto.
+    intros [i''' [s2''' [P Q]]].
+    (* Exploit determinacy *)
+    exploit @f2b_determinacy_star. 1-2: eauto.
+    eauto. eexact STEP2. auto. apply plus_star; eauto.
+    intro R. inv R. congruence.
+    exploit not_silent_length. eapply (sr_traces L1_receptive); eauto. intros [EQ | EQ].
+    subst. simpl in *. exploit @sd_determ_1. eauto. eexact STEP2. eexact H2.
+    intros. elim NOT2. inv H7; auto.
+    subst. rewrite E0_right in *.
+    assert (s3 = s2'). eapply sd_determ_2; eauto. subst s3.
+    (* Perform transition now and go to "after" state *)
+    destruct (star_starN H6) as [n STEPS2]. exists (F2BI_after n); exists s1'''; split.
+    left. apply plus_one; auto.
+    eapply f2b_pmatch_normal.
+    eapply f2b_match_after'; eauto.
+
+- (* 3. After *)
+  inv H. exploit Eapp_E0_inv; eauto. intros [EQ1 EQ2]; subst.
+  exploit @f2b_determinacy_inv. 1-2: eauto. eexact H2. eexact STEP2.
+  intros [[EQ1 [EQ2 EQ3]] | [NOT1 [NOT2 MT]]].
+  subst. exists (F2BI_after n); exists s1; split.
+  right; split. apply star_refl. constructor; lia.
+  eapply f2b_pmatch_normal.
+  eapply f2b_match_after'; eauto.
+  congruence.
+  
+(* 4. Error states *)
+- inv STARN.
+  (* impossible: error state s2a cannot take a step *)
+  exfalso. eapply sd_err_nostep; eauto.
+  exploit @f2b_determinacy_inv. 1-2: eauto. eexact H. eexact STEP2.
+  intros [[EQ1 [EQ2 EQ3]] | [NOT1 [NOT2 MT]]].
+  + (* 4.1 L2 makes a silent transition: remain in "before" state *)
+    subst. simpl in *. exists (F2BI_before n0); exists s1; split.
+    right; split. apply star_refl. constructor. lia.
+    subst. eapply f2b_pmatch_err; eauto.
+    eapply star_right; eauto.
+  + exploit Eapp_E0_inv; eauto.
+    intros (A1 & A2). subst. congruence.
+    
+Qed.
+
+End FORWARD_TO_BACKWARD.
+
+Lemma forward_to_backward_simulation_partial:
+  forall {liA1 liA2} (ccA: callconv liA1 liA2),
+  forall {liB1 liB2} (ccB: callconv liB1 liB2),
+  forall L1 L2 err_state1 err_state2,
+    forward_simulation_ppub ccA ccB L1 L2 err_state1 err_state2 ->
+    receptive L1 ->
+    determinate L2 ->
+    sound_err L2 err_state2 ->
+    backward_simulation_preserve_error ccA ccB L1 L2 err_state1 err_state2.
+Proof.
+  intros until err_state2. intros FS L1_receptive L2_determinate Err2.
+  destruct FS as [[index order match_states Hskel FS order_wf]].
+  set (ms se1 se2 w := f2b_partial_match_states (L1 se1) (L2 se2) (match_states := match_states se1 se2 w) (err_state1 se1) (err_state2 se2)).
+  constructor.
+  eapply Backward_simulation_preserve_error with f2b_order ms; auto using wf_f2b_order.
+  intros se1 se2 wB Hse Hse1.
+  specialize (FS se1 se2 wB Hse Hse1).
+  specialize (L1_receptive se1). specialize (L2_determinate se2).
+  specialize (Err2 se2).
+  inv FS.
+  split. 
+- (* valid queries *)
+  eapply fsim_match_valid_query; eauto.
+- split.
+  (* initial states exist *)
+  intros. exploit (fsim_match_initial_states fsimp_prop0); eauto. intros [i [s2 [A B]]].
+  exists s2; auto.
+  (* initial states *)
+  intros. exploit (fsim_match_initial_states fsimp_prop0); eauto. intros [i [s2' [A B]]].
+  assert (s2 = s2') by (eapply sd_initial_determ; eauto). subst s2'.
+  exists s1; split; auto. exists (F2BI_after O). econstructor; eauto.
+  econstructor; eauto.
+- (* final states *)
+  intros. inv H. inv MATCH.
+  + exploit @f2b_partial_progress; eauto. intros TRANS; inv TRANS. inv H2.
+    * assert (r0 = r2) by eauto using sd_final_determ; subst. eauto using star_refl.
+    * eelim sd_final_noext; eauto.
+    * inv H5. exploit (sd_final_nostep L2_determinate); eauto. contradiction.
+    * inv H5.
+      -- (* final no error *)
+        exfalso. eapply sd_final_noerr; eauto.
+      -- exploit (sd_final_nostep L2_determinate); eauto. contradiction.
+  + inv H4. congruence. exploit (sd_final_nostep L2_determinate); eauto. contradiction.
+  + inv H. exploit (sd_final_nostep L2_determinate); eauto. contradiction.
+  + inv STARN.
+    * (* final no error *)
+      exfalso. eapply sd_final_noerr; eauto.
+    * exploit (sd_final_nostep L2_determinate); eauto. contradiction.
+- (* external states *)
+  intros. inv H. inv MATCH.
+  + exploit @f2b_partial_progress; eauto.
+    intros TRANS; inv TRANS. inv H2.
+    * eelim (sd_final_noext L2_determinate); eauto.
+    * assert (q0 = q2) by eauto using sd_at_external_determ; subst.
+      exists wA, s1', q1. intuition auto. split.
+      intros. edestruct H8 as (j & s2' & Hs2' & Hs'); eauto.
+      intros. edestruct H8 as (j & s2' & Hs2' & Hs'); eauto.
+      assert (s3 = s2') by eauto using sd_after_external_determ; subst.
+      exists s0. intuition auto.
+      exists (F2BI_after O). econstructor; eauto. econstructor; eauto.
+    * inv H5. eelim (sd_at_external_nostep L2_determinate); eauto.
+    * inv H5.
+      -- (* external no error *)
+        exfalso. eapply sd_external_noerr; eauto.
+      -- eelim (sd_at_external_nostep L2_determinate); eauto.
+  + inv H4. congruence. eelim (sd_at_external_nostep L2_determinate); eauto.
+  + inv H. eelim (sd_at_external_nostep L2_determinate); eauto.
+  + inv STARN.
+    -- (* external no error *)
+      exfalso. eapply sd_external_noerr; eauto.
+    -- eelim (sd_at_external_nostep L2_determinate); eauto.
+- (* progress *)
+  intros. inv H. inv MATCH.
+  + exploit @f2b_partial_progress; eauto. intros TRANS; inv TRANS; inv H1; eauto.
+    * inv H4. left. eauto.
+    * inv H4; eauto.
+      left. eauto.
+    * inv H4; eauto.
+      left. eauto.
+  + inv H3; eauto. congruence.
+    left. eauto.
+  + inv H. left. eauto.
+  + inv STARN; eauto.
+    left. eauto.
+- (* simulation *)
+  eapply f2b_simulation_step; eauto.
+Qed.
